io/DM.IIO.Primitives.fst
@@ -2,31 +2,34 @@ module DM.IIO.Primitives
 
 open FStar.Tactics
 open ExtraTactics
-open DM.IIO.Tactics
 open FStar.Tactics.Typeclasses
+open DM.IIO.Tactics
 
 open Common
-open Free.IO
+open IO.Sig
 open DM.IO
 open DM.IIO
+open TC.Checkable
 open TC.Trivialize.IIOwp
 
 val dynamic_cmd :
   (cmd : io_cmds) ->
-  (pi : monitorable_prop) ->
-  (arg : args cmd) ->
-  IIOwp (maybe (io_resm cmd)) (fun h p ->
-    (forall (r:maybe (io_resm cmd)) lt.
-      ((match r with
-      | Inr Contract_failure -> lt == []
-      | Inl r' -> lt == [convert_call_to_event cmd arg r']
-      | _ -> False) /\
-      enforced_locally pi h lt) ==> p r lt))
-let dynamic_cmd (cmd:io_cmds) = 
+  (d1 : checkable2 (io_pre cmd)) ->
+  (arg : io_sig.args cmd) ->
+  IIOwp (maybe (io_resm cmd)) 
+    (fun p h ->
+      (forall (r:maybe (io_sig.res cmd arg)) lt.
+        (match r with
+         | Inr Contract_failure -> lt == []
+         | Inl r' -> lt == [convert_call_to_event cmd arg r']
+         | _ -> False) ==> p lt r))
+let dynamic_cmd (cmd:io_cmds) d1 = 
   trivialize 
     #_ 
-    #(trivializeable_IIOwp_2 monitorable_prop (args cmd) _
-      (fun pi argz h -> pi h (| cmd, argz |))
-      (fun pi argz h r lt -> 
-        lt == [convert_call_to_event cmd argz r] /\ enforced_locally pi h lt))
+    #(trivializeable_IIOwp
+       (io_sig.args cmd)
+       (io_resm cmd)
+       (io_pre cmd)
+       #d1
+       (fun (argz:io_sig.args cmd) h r lt -> lt == [convert_call_to_event cmd argz r]))
   (static_cmd cmd)
