io/DM.fst
@@ -1,6 +1,6 @@
 module DM
 
-include Free.IO
+include IO.Sig
 include DM.IO
 include DM.IIO
 include DM.IIO.Primitives
